<?xml version="1.0"?>
<rdf:RDF xmlns="http://www.semanticweb.org/ilbuonme/ontologies/2020/6/graphematics#"
     xml:base="http://www.semanticweb.org/ilbuonme/ontologies/2020/6/graphematics"
     xmlns:dc="http://purl.org/dc/elements/1.1/"
     xmlns:owl="http://www.w3.org/2002/07/owl#"
     xmlns:rdf="http://www.w3.org/1999/02/22-rdf-syntax-ns#"
     xmlns:xml="http://www.w3.org/XML/1998/namespace"
     xmlns:xsd="http://www.w3.org/2001/XMLSchema#"
     xmlns:rdfs="http://www.w3.org/2000/01/rdf-schema#"
     xmlns:skos="http://www.w3.org/2004/02/skos/core#">
    <owl:Ontology rdf:about="https://graphematics.vedph.it/graphematics">
        <owl:versionIRI rdf:resource="https://graphematics.vedph.it/graphematics/1.0.0"/>
        <rdfs:comment xml:lang="en">Ontology for concepts pertaining to graphemes and writing systems, oriented to philology.

This is work in progress: it is being actively developed as of summer 2020.

Three closely related ontologies, to which this ontology will eventually be intertwined, are
- Peter Stokes, [The Archetype Ontology](https://github.com/pastokes/archetype-ontology)
- [CRMtex](http://www.cidoc-crm.org/crmtex/sites/default/files/CRMtex_v1.0_March_2020.pdf)
- Frekerike Neuber, [typoo](https://github.com/FrederikeNeuber/typoo/)</rdfs:comment>
        <rdfs:label>POGO, Philology-oriented graphematics ontology</rdfs:label>
    </owl:Ontology>
    


    <!-- 
    ///////////////////////////////////////////////////////////////////////////////////////
    //
    // Annotation properties
    //
    ///////////////////////////////////////////////////////////////////////////////////////
     -->

    


    <!-- http://purl.org/dc/elements/1.1/creator -->

    <owl:AnnotationProperty rdf:about="http://purl.org/dc/elements/1.1/creator"/>
    


    <!-- 
    ///////////////////////////////////////////////////////////////////////////////////////
    //
    // Object Properties
    //
    ///////////////////////////////////////////////////////////////////////////////////////
     -->

    


    <!-- http://erlangen-crm.org/current/P138_represents -->

    <owl:ObjectProperty rdf:about="http://erlangen-crm.org/current/P138_represents">
        <owl:inverseOf rdf:resource="http://erlangen-crm.org/current/P138i_is_represented_by"/>
    </owl:ObjectProperty>
    


    <!-- http://erlangen-crm.org/current/P138i_is_represented_by -->

    <owl:ObjectProperty rdf:about="http://erlangen-crm.org/current/P138i_is_represented_by"/>
    


    <!-- http://erlangen-crm.org/current/P65i_is_shown_by -->

    <owl:ObjectProperty rdf:about="http://erlangen-crm.org/current/P65i_is_shown_by">
        <owl:inverseOf rdf:resource="http://erlangen-crm.org/current/E1_CRM_Entity#P65_shows_visual_item"/>
    </owl:ObjectProperty>
    


    <!-- http://erlangen-crm.org/current/E1_CRM_Entity#P65_shows_visual_item -->

    <owl:ObjectProperty rdf:about="http://erlangen-crm.org/current/E1_CRM_Entity#P65_shows_visual_item"/>
    


    <!-- https://graphematics.vedph.it/graphematics#POGO_has_standard_alphabetic_meaning -->

    <owl:ObjectProperty rdf:about="https://graphematics.vedph.it/graphematics#POGO_has_standard_alphabetic_meaning">
        <owl:inverseOf rdf:resource="https://graphematics.vedph.it/graphematics#POGO_is_standard_alphabetic_meaning_of"/>
    </owl:ObjectProperty>
    


    <!-- https://graphematics.vedph.it/graphematics#POGO_is_standard_alphabetic_meaning_of -->

    <owl:ObjectProperty rdf:about="https://graphematics.vedph.it/graphematics#POGO_is_standard_alphabetic_meaning_of"/>
    


    <!-- 
    ///////////////////////////////////////////////////////////////////////////////////////
    //
    // Classes
    //
    ///////////////////////////////////////////////////////////////////////////////////////
     -->

    


    <!-- http://erlangen-crm.org/current/E37_Mark -->

    <owl:Class rdf:about="http://erlangen-crm.org/current/E37_Mark">
        <rdfs:subClassOf rdf:resource="http://erlangen-crm.org/current/E90_Symbolic_Object"/>
    </owl:Class>
    


    <!-- http://erlangen-crm.org/current/E90_Symbolic_Object -->

    <owl:Class rdf:about="http://erlangen-crm.org/current/E90_Symbolic_Object"/>
    


    <!-- http://www.cidoc-crm.org/crmtex/TX8_Grapheme -->

    <owl:Class rdf:about="http://www.cidoc-crm.org/crmtex/TX8_Grapheme">
        <rdfs:subClassOf rdf:resource="http://erlangen-crm.org/current/E90_Symbolic_Object"/>
    </owl:Class>
    


    <!-- http://www.cidoc-crm.org/crmtex/TX9_Glyph -->

    <owl:Class rdf:about="http://www.cidoc-crm.org/crmtex/TX9_Glyph">
        <rdfs:subClassOf rdf:resource="http://erlangen-crm.org/current/E37_Mark"/>
        <rdfs:subClassOf>
            <owl:Restriction>
                <owl:onProperty rdf:resource="http://erlangen-crm.org/current/E1_CRM_Entity#P65_shows_visual_item"/>
                <owl:qualifiedCardinality rdf:datatype="http://www.w3.org/2001/XMLSchema#nonNegativeInteger">1</owl:qualifiedCardinality>
                <owl:onClass rdf:resource="https://graphematics.vedph.it/graphematics#Allograph"/>
            </owl:Restriction>
        </rdfs:subClassOf>
        <rdfs:comment xml:lang="en">The definition of &apos;crm:P62 depicts&apos; says: &quot;This property is a shortcut of the more fully developed path from E24 Physical Human-Made Thing through P65 shows visual item, E36 Visual Item, P138 represents, E1 CRM Entity&quot;.

CRMtex asserts that TX9 Glyph, P62 depicts, TX8 Grapheme. This is equivalent to TX9 Glyph (a E24 Physical Human-Made Thing), P65 shows visual item, something unspecified (a E36 Visual Item), P138 represents, TX8 Grapheme (a E1 CRM Entity). Here one position in the chain (the E46 Visual Item) is unspecified.

So when this ontology asserts that TX9 Glyph (a E24 Physical Human-Made Thing), P65 shows visual item, POGO_Allograph (a E37 Mark, which is a E36 Visual Item), P138 represents, TX8 Grapheme (a E1 CRM Entity)&quot;, this ontology is not contradicting CRMtex but integrating it, by adding POGO_Allograph in the empty position in the chain (the E46 Visual Item).</rdfs:comment>
    </owl:Class>
    


    <!-- https://graphematics.vedph.it/graphematics#Abbreviation -->

    <owl:Class rdf:about="https://graphematics.vedph.it/graphematics#Abbreviation">
        <rdfs:subClassOf rdf:resource="http://erlangen-crm.org/current/E90_Symbolic_Object"/>
        <rdfs:label xml:lang="en">POGO_Abbreviation</rdfs:label>
    </owl:Class>
    


    <!-- https://graphematics.vedph.it/graphematics#Abbreviation_Mark -->

    <owl:Class rdf:about="https://graphematics.vedph.it/graphematics#Abbreviation_Mark">
        <rdfs:subClassOf rdf:resource="https://graphematics.vedph.it/graphematics#Segmental_Grapheme"/>
        <rdfs:comment xml:lang="en">Property +{alphabetic}, i.e. does have function to [Alphabeme]+ (1 or more [Alphabeme]).

Property +{has_a_1_to_1_standard_alphabetic_meaning}, i.e. there is one Alphabeme (not Phoneme) wich it represents its standard alphabetic meaning.

Properties:
{+linguistic}
{+intraverbal}
{+alphabetic}
{-has_a_1_to_1_standard_alphabetic_meaning}
{+combining}

Examples: macron, semicolon, dot and other graphemes written to mark an abbreviation.

Example of property {+alphabetic}: in &apos;mīa&apos; (abbreviated form for &apos;misericordia&apos;), the four grahemes &apos;m&apos;, &apos;i&apos;, &apos;a&apos; and macron (which can span over the whole graphical word or over a part of it), combined, have function to the alphabemes &apos;m&apos;, &apos;i&apos;, &apos;s&apos;, &apos;e&apos; etc.</rdfs:comment>
        <rdfs:label xml:lang="en">POGO_Abbreviation_Mark</rdfs:label>
    </owl:Class>
    


    <!-- https://graphematics.vedph.it/graphematics#Allograph -->

    <owl:Class rdf:about="https://graphematics.vedph.it/graphematics#Allograph">
        <rdfs:subClassOf rdf:resource="http://erlangen-crm.org/current/E37_Mark"/>
        <rdfs:subClassOf>
            <owl:Restriction>
                <owl:onProperty rdf:resource="http://erlangen-crm.org/current/P138_represents"/>
                <owl:qualifiedCardinality rdf:datatype="http://www.w3.org/2001/XMLSchema#nonNegativeInteger">1</owl:qualifiedCardinality>
                <owl:onClass rdf:resource="http://www.cidoc-crm.org/crmtex/TX8_Grapheme"/>
            </owl:Restriction>
        </rdfs:subClassOf>
        <rdfs:comment xml:lang="en">A POGO_Allograph is a CRM &apos;E37 Mark&apos;, which in its turn is a CRM &apos;E36 Visual Item&apos;.  The definition of crm:E37 says that &quot;Instances of E37 Mark do not represent the actual image of a mark, but the abstract ideal&quot;. Likewise, the definition of crm:E36 says that &quot; This class does not intend to describe the idiosyncratic characteristics of an individual physical embodiment of a visual item, but the underlying prototype&quot;. A POGO_Allograph is the abstract form, the visual model, which scribes have in mind when drawing (and readers have in mind when recognizing) individual TX9 Glyphs. No two TX9 Glyphs are identical, but all TX9 Glyphs that P65_shows_visual_item the same POGO_Allograph are modelled on the same abstract form, that of the POGO_Allograph.

It is important to note that while both a TX9 Glyph and a POGO_Allograph are &apos;visual&apos; in that they have a form, a shape (a Glyph has a specific, unique shape, an Allograph is an abstract model), in this ontology a TX8 Grapheme does not have a shape. For example, while POGO_Allograph &apos;ſ&apos; (long s) has an oblong shape with a hook at its top and the shape of POGO_Allograph &apos;s&apos; (short s) is characterized by two curves, TX8 Grapheme &apos;s&apos; does not have any shape. If it did, what would it be: the oblong one or the double-curve one?

The POGO ontology and Peter Stokes&apos; Archetype ontology have different perspective: POGO is oriented towards philology, so it considers concepts within one writing system, i.e. within each hand of each handwritten document; Archetype is oriented towards paleography, so it considers concepts across different hands. As a consequence, an Archetype_Idiograph also corresponds to a POGO_Allograph, if that is the only shape which that specific hand knows. In Archetype&apos;s perspective, there is such a thing as &apos;long s Archetype_allograph that is the same in different manuscript hands, and there is a specific Archetype_idiograph &apos;long s 1&apos; of that Archetype_allograph in hand &apos;a&apos; of manuscript &apos;A&apos; and a different Archetype_idiograph &apos;long s 2&apos; of that Archetype_allograph in hand &apos;b&apos; of manuscript &apos;B&apos;. For POGO instead, when editing manuscript A, one considers &apos;long s&apos; (shaped with the specific shape of &apos;long s 1&apos;) as a POGO_Allograph of POGO-Gapheme &apos;s&apos; within the writing system of hand &apos;a&apos; of manuscript &apos;A&apos;, and the same for the corresponding allograph in the writing system of hand &apos;b&apos; of manuscript &apos;B&apos;.

Open issue: strictly speaking, the term &apos;Allograph&apos; should only be used when in a writing system more than one abstract visual form exist for a grapheme (like the ſ/s example above). However, in this ontology the term is also used to refer to the abstract model of TX9 Glyphs in the case in which in a writing system only one allograph exists for a grapheme. This clashes with the etymological meaning of morpheme &apos;allo-&apos; (other) in the class name POGO_Allograph. An alternative name for this class would have been &apos;Graph&quot;, as suggested privately both by Raul Mordenti and Frederike Neuber.</rdfs:comment>
        <rdfs:label xml:lang="en">POGO_Allograph</rdfs:label>
    </owl:Class>
    


    <!-- https://graphematics.vedph.it/graphematics#Alphabeme -->

    <owl:Class rdf:about="https://graphematics.vedph.it/graphematics#Alphabeme">
        <rdfs:subClassOf rdf:resource="http://erlangen-crm.org/current/E90_Symbolic_Object"/>
        <rdfs:comment>Minimal distinctive unit of an alphabet. It does not have a shape model and may be represented by a grapheme, by a signal of the Morse code, by a sequence of phonemes, by a sign in the deaf sign language etc. It relationship with the Phoneme is complex and variable.</rdfs:comment>
        <rdfs:label xml:lang="en">POGO_Alphabeme</rdfs:label>
    </owl:Class>
    


    <!-- https://graphematics.vedph.it/graphematics#Alphabetic_Grapheme -->

    <owl:Class rdf:about="https://graphematics.vedph.it/graphematics#Alphabetic_Grapheme">
        <rdfs:subClassOf rdf:resource="https://graphematics.vedph.it/graphematics#Segmental_Grapheme"/>
        <rdfs:subClassOf>
            <owl:Restriction>
                <owl:onProperty rdf:resource="https://graphematics.vedph.it/graphematics#POGO_has_standard_alphabetic_meaning"/>
                <owl:qualifiedCardinality rdf:datatype="http://www.w3.org/2001/XMLSchema#nonNegativeInteger">1</owl:qualifiedCardinality>
                <owl:onClass rdf:resource="https://graphematics.vedph.it/graphematics#Alphabeme"/>
            </owl:Restriction>
        </rdfs:subClassOf>
        <rdfs:comment xml:lang="en">Property +{alphabetic}, i.e. does have function to [Alphabeme]+ (1 or more [Alphabeme]).

Property +{has_a_1_to_1_standard_alphabetic_meaning}, i.e. there is one Alphabeme (not Phoneme) wich it represents its standard alphabetic meaning.

Problematic aspect: some Alphabetic Graphemes (that I would call &apos;Combining Alphabetic Graphemes&apos;) can be put above or below another Alphabetic Grapheme, or &apos;Base Alphabetic Grapheme&apos; (e.g. a small &apos;o&apos; over an &apos;u&apos; or, in Greek, a small iota under an omega), thus being used as abbreviations. The same happens today in superscript such as 1st or 2nd in English, or 1° in Italian (for &apos;primo&apos;).

Properties:
{+linguistic}
{+intraverbal}
{+alphabetic}

Base Alphabetic Graphemes also have properties:
{-combining}

Combining Alphabetic Graphemes also have properties:
{+combining}

Examples include: &apos;a&apos;, &apos;b&apos;, &apos;c&apos;... for graphemes referring to alphabemes of the Latin alphabet; alpha, beta, gamma... for those referring to the Greek alphabet.</rdfs:comment>
        <rdfs:label xml:lang="en">POGO_Alphabetic_Grapheme</rdfs:label>
    </owl:Class>
    


    <!-- https://graphematics.vedph.it/graphematics#Brevigraph -->

    <owl:Class rdf:about="https://graphematics.vedph.it/graphematics#Brevigraph">
        <rdfs:subClassOf rdf:resource="https://graphematics.vedph.it/graphematics#Segmental_Grapheme"/>
        <rdfs:subClassOf>
            <owl:Restriction>
                <owl:onProperty rdf:resource="https://graphematics.vedph.it/graphematics#POGO_has_standard_alphabetic_meaning"/>
                <owl:minQualifiedCardinality rdf:datatype="http://www.w3.org/2001/XMLSchema#nonNegativeInteger">2</owl:minQualifiedCardinality>
                <owl:onClass rdf:resource="https://graphematics.vedph.it/graphematics#Alphabeme"/>
            </owl:Restriction>
        </rdfs:subClassOf>
        <rdfs:comment xml:lang="en">One Grapheme meaning more than one Alphabeme.

Property +{alphabetic}, i.e. does have function to [Alphabeme]+ (1 or more [Alphabeme]).

Property +{has_a_1_to_1_standard_alphabetic_meaning}, i.e. there is one Alphabeme (not Phoneme) wich it represents its standard alphabetic meaning.

Properties:
{+linguistic}
{+intraverbal}
{+alphabetic}
{-has_a_1_to_1_standard_alphabetic_meaning}
{-combining}

Examples include: p with horizontal trait for Latin &quot;per&quot;, q with horizontal trait for lat. &quot;qui&quot; etc.

Problematic aspect: brevigraphs mostly derive from original graphemes (&apos;p&apos;, &apos;q&apos;, &apos;e&apos; etc.) with modifications. In some cases, such as the &apos;e caudatum&apos; (originating from a ligature between &apos;a&apos; and &apos;e&apos;) or the &apos;4-shaped&apos; abbreviation for final &apos;-rum&apos; in Latin (bonorum etc.), the original graphemes have fused in such a manner that one would hardly distinguish them any more. In other cases, instead, the original traits are easily distinguishable, so one could analyze &apos;p with horizontal trait&apos; as two distinct graphemes, &apos;p&apos; and &apos;horizontal trait&apos;. This relates to the very issue of the definition of grapheme as &apos;minimal&apos; unit.</rdfs:comment>
        <rdfs:label xml:lang="en">POGO_Brevigraph</rdfs:label>
    </owl:Class>
    


    <!-- https://graphematics.vedph.it/graphematics#Diacritic -->

    <owl:Class rdf:about="https://graphematics.vedph.it/graphematics#Diacritic">
        <rdfs:subClassOf rdf:resource="https://graphematics.vedph.it/graphematics#Segmental_Grapheme"/>
        <rdfs:comment xml:lang="en">Property -{alphabetic}, i.e. doesn&apos;t have function to [Alphabeme]+ (1 or more [Alphabeme]).

Properties:
{+linguistic}
{+intraverbal}
{-alphabetic}
{+combining}

Examples include: accent, macron meaning long vowel.

Its distinction with textual graphemes, and possibly also with abbreviation marks, may be blurred in practice.

A diacritic dffers from graphemes having +{alphabetic} such as the abbreviation mark because, for instance, we do not consider the &apos;o&apos; in Italian words &apos;pero&apos; and &apos;però&apos; as distinct alphabemes, while the alphabeme sequences in &apos;lacu&apos; (ablative) and &apos;lacū&apos; (abbreviation for accusative &apos;lacum&apos;) do differ because of the macron (abbreviation mark).

The main distinction between a diacritic and a textual graphemes is that a diacritic is considered as part of one word, referring to the whole word or to individual graphemes within it, while a textual grapheme like a comma does not refer to one word, but has function to a number of words, and in principle has function to the whole text.</rdfs:comment>
        <rdfs:label xml:lang="en">POGO_Diacritic</rdfs:label>
    </owl:Class>
    


    <!-- https://graphematics.vedph.it/graphematics#Glottographic_Grapheme -->

    <owl:Class rdf:about="https://graphematics.vedph.it/graphematics#Glottographic_Grapheme">
        <rdfs:subClassOf rdf:resource="http://www.cidoc-crm.org/crmtex/TX8_Grapheme"/>
        <rdfs:comment xml:lang="en">A Grapheme meaning a word or a part of it. The name and the concept are taken from G. Sampson, Writing Systems, pp. 38-39.</rdfs:comment>
        <rdfs:label xml:lang="en">POGO_Glottographic_Grapheme</rdfs:label>
    </owl:Class>
    


    <!-- https://graphematics.vedph.it/graphematics#Segmental_Grapheme -->

    <owl:Class rdf:about="https://graphematics.vedph.it/graphematics#Segmental_Grapheme">
        <rdfs:subClassOf rdf:resource="https://graphematics.vedph.it/graphematics#Glottographic_Grapheme"/>
        <rdfs:comment xml:lang="en">A grapheme that is part of a word (or morpheme). These graphemes correspond to the second articulation of language. Though they normally belong to &apos;phonographic&apos; writing systems (G. Sampson, Writing Systems, pp. 39-45 distinguishes three kinds of phonographic systems: syllabic, segmental and featural), I want to hightlight that one intraverbal grapheme does not necessarily represent one phoneme. Writing systems are independent semiotic systems, constituting a &apos;manifestation&apos; of the abstract structures of the language (Hjelmslev, Prolegomena to a Theory of Language, chapter 21, &apos;Language and non-language&apos;) distinct from the &apos;manifestation&apos; of those structures represented by spoken language. There relationship between intraverbal graphemes and phonemes is complex: examples  of this complexity include diacritics, abbreviation marks and brevigraphs, but also an alphabetic grapheme such as &apos;h&apos;, to which no phoneme corresponds in the pronunciation in some languages (like Italian); and another alphabetic grapheme such as &apos;c&apos;, to which many pronunciations corresponded in Latin throughout social classes, time and space.</rdfs:comment>
        <rdfs:label xml:lang="en">POGO_Segmental_Grapheme</rdfs:label>
    </owl:Class>
    


    <!-- https://graphematics.vedph.it/graphematics#Ligature -->

    <owl:Class rdf:about="https://graphematics.vedph.it/graphematics#Ligature">
        <rdfs:subClassOf rdf:resource="http://erlangen-crm.org/current/E90_Symbolic_Object"/>
        <rdfs:label xml:lang="en">POGO_Ligature</rdfs:label>
    </owl:Class>
    


    <!-- https://graphematics.vedph.it/graphematics#Logograph -->

    <owl:Class rdf:about="https://graphematics.vedph.it/graphematics#Logograph">
        <rdfs:subClassOf rdf:resource="https://graphematics.vedph.it/graphematics#Glottographic_Grapheme"/>
        <rdfs:comment>A Grapheme meaning a whole word or a morpheme. The name and the concept are taken from G. Sampson, Writing Systems, pp. 38-39. It is worth quoting from page 39: &quot;[...] one might imagine a logographic script for English in which, say, the words walk, walked, walking were represented by three distinct and unrelted graphs, rather than being split into their constituent morphemes [...]. In reality, though, I know of no logographic systems based on units larger than single morphemes&quot;. Bear in mind that word roots (e.g. &quot;dog&quot;) also are &quot;morphemes&quot;.</rdfs:comment>
        <rdfs:label xml:lang="en">POGO_Logograph</rdfs:label>
    </owl:Class>
    


    <!-- https://graphematics.vedph.it/graphematics#Metamark -->

    <owl:Class rdf:about="https://graphematics.vedph.it/graphematics#Metamark">
        <rdfs:subClassOf rdf:resource="https://graphematics.vedph.it/graphematics#Textual_Grapheme"/>
        <rdfs:comment>This class includes textual graphemes that do not qualify as space or punctuation, such as an asterisk pointing to a footnote, a mark in a manuscript pointing to an interlinear or a marginal addition. This class might be eliminated in future versions of the ontology, since it mostly represents &apos;other textual graphemes&apos; (not being space or proper punctuation). However, such metamarks have specific markup conventions in TEI.</rdfs:comment>
        <rdfs:label xml:lang="en">POGO_Metamark</rdfs:label>
    </owl:Class>
    


    <!-- https://graphematics.vedph.it/graphematics#Punctuation_Mark -->

    <owl:Class rdf:about="https://graphematics.vedph.it/graphematics#Punctuation_Mark">
        <rdfs:subClassOf rdf:resource="https://graphematics.vedph.it/graphematics#Textual_Grapheme"/>
        <rdfs:comment>Examples include comma, full stop, question mark, quotes. Especially in pre-modern writing systems, the status of some textual graphemes (such as asterisks or the obelos in ancient Greek papyri) is controversial: some would call them punctuation, some not. So the distinction between current classes &quot;Punctuation Mark&quot; and &quot;Metamark&quot; is blurred in practice. In other words, punctuation has been standardized for Western writing systems only in the contemporary age, and its status in other writing systems is still problematic.</rdfs:comment>
        <rdfs:label xml:lang="en">POGO_Punctuation_Mark</rdfs:label>
    </owl:Class>
    


    <!-- https://graphematics.vedph.it/graphematics#Semasiographic_Grapheme -->

    <owl:Class rdf:about="https://graphematics.vedph.it/graphematics#Semasiographic_Grapheme">
        <rdfs:subClassOf rdf:resource="http://www.cidoc-crm.org/crmtex/TX8_Grapheme"/>
        <rdfs:comment>A Grapheme meaning an idea, not a word. The name and the concept are taken from G. Sampson, Writing Systems, pp. 28-38. This covers the concept sometimes called ideogram or pictogram. Examples include numbers and Chinese characters.</rdfs:comment>
        <rdfs:label xml:lang="en">POGO_Semasiographic_Grapheme</rdfs:label>
    </owl:Class>
    


    <!-- https://graphematics.vedph.it/graphematics#Space -->

    <owl:Class rdf:about="https://graphematics.vedph.it/graphematics#Space">
        <rdfs:subClassOf rdf:resource="https://graphematics.vedph.it/graphematics#Textual_Grapheme"/>
        <rdfs:comment>Examples include &apos;white&apos; space between graphical words and other uses of space to arrange marks on the page, such as line breaks. In a written document produced with ink &quot;Space&quot; is not produced directly by adding ink, but instead by arranging other marks in a specific way, so one could argue that &quot;Space&quot; is not a subclass of &quot;Mark&quot;, but I would still argue that it is a subclass of &quot;Grapheme&quot; because it has distinctive value. Its status is therefore quite unique and problematic.</rdfs:comment>
        <rdfs:label xml:lang="en">POGO_Space</rdfs:label>
    </owl:Class>
    


    <!-- https://graphematics.vedph.it/graphematics#Textual_Grapheme -->

    <owl:Class rdf:about="https://graphematics.vedph.it/graphematics#Textual_Grapheme">
        <rdfs:subClassOf rdf:resource="http://www.cidoc-crm.org/crmtex/TX8_Grapheme"/>
        <rdfs:comment>A Grapheme used as a metalanguage providing a meaningful syntax for other graphemes in the text. It does not distinguish between different words but between different texts.</rdfs:comment>
        <rdfs:label xml:lang="en">POGO_Textual_Grapheme</rdfs:label>
    </owl:Class>
</rdf:RDF>



<!-- Generated by the OWL API (version 4.5.9.2019-02-01T07:24:44Z) https://github.com/owlcs/owlapi -->

